pulse/lib/steel/pulse/Pulse.Checker.Comp.fsti
@@ -20,8 +20,9 @@ module T = FStar.Tactics.V2
 
 open Pulse.Syntax
 open Pulse.Typing
+open Pulse.Typing.Metatheory.Base
 
 val check (g:env) 
           (c:comp_st)
           (pre_typing:tot_typing g (comp_pre c) tm_vprop)
-  : T.Tac (comp_typing g c (comp_u c))
+  : T.Tac (comp_typing g c (universe_of_comp c))
