pulse/lib/steel/pulse/Pulse.Checker.If.fst
@@ -68,12 +68,12 @@ let lift_ghost_to_atomic
          (ensures fun (| c', _ |) ->
              st_comp_of_comp c' == st_comp_of_comp c /\
              ctag_of_comp_st c' == STT_Atomic /\
-             C_STGhost?.inames c == C_STAtomic?.inames c')
-= let C_STGhost inames c_st = c in
+             tm_emp_inames == C_STAtomic?.inames c')
+= let C_STGhost c_st = c in
   let w = get_non_informative_witness g (comp_u c) (comp_res c) in
-  let c' = C_STAtomic inames Unobservable c_st in
+  let c' = C_STAtomic tm_emp_inames Neutral c_st in
   let d' : st_typing g e c' =
-    T_Lift g e c c' d (Lift_STGhost_STUnobservable g c w)
+    T_Lift g e c c' d (Lift_Ghost_Neutral g c w)
   in
   (| c', d' |)
 
@@ -99,7 +99,7 @@ let lift_if_branches
             ctag_of_comp_st c_then' == ctag_of_comp_st c_else')
 = let g = g_then in
   match c_then, c_else with
-  | C_STGhost _ _, C_STGhost _ _ 
+  | C_STGhost _, C_STGhost _ 
   | C_STAtomic _ _ _, C_STAtomic _ _ _
   | C_ST _, C_ST _ ->
     (* Nothing to do *)
@@ -113,35 +113,35 @@ let lift_if_branches
     let (| c_else', e_else_typing' |) = lift_atomic_to_st g_else e_else c_else e_else_typing in
     (| c_then, c_else', e_then_typing, e_else_typing' |)
 
-  | C_STGhost _ _, C_STAtomic _ _ _ ->
+  | C_STGhost _, C_STAtomic _ _ _ ->
     let (| c_then', e_then_typing' |) = lift_ghost_to_atomic g_then e_then c_then e_then_typing in
     (| c_then', c_else, e_then_typing', e_else_typing |)
 
-  | C_STAtomic _ _ _, C_STGhost _ _ ->
+  | C_STAtomic _ _ _, C_STGhost _ ->
     let (| c_else', e_else_typing' |) = lift_ghost_to_atomic g_else e_else c_else e_else_typing in
     (| c_then, c_else', e_then_typing, e_else_typing' |)
 
-  | C_STGhost _ _, C_ST _ ->
+  | C_STGhost _, C_ST _ ->
     let (| c_then', e_then_typing' |) = lift_ghost_to_atomic g_then e_then c_then  e_then_typing  in
     let (| c_then', e_then_typing' |) = lift_atomic_to_st    g_then e_then c_then' e_then_typing' in
     (| c_then', c_else, e_then_typing', e_else_typing |)
 
-  | C_ST _, C_STGhost _ _ ->
+  | C_ST _, C_STGhost _ ->
     let (| c_else', e_else_typing' |) = lift_ghost_to_atomic g_else e_else c_else  e_else_typing  in
     let (| c_else', e_else_typing' |) = lift_atomic_to_st    g_else e_else c_else' e_else_typing' in
     (| c_then, c_else', e_then_typing, e_else_typing' |)
 
 let inames_of_comp (c:comp_st) : term =
   match c with
-  | C_ST _ -> tm_emp_inames
+  | C_ST _
+  | C_STGhost _ -> tm_emp_inames
   | C_STAtomic inames _ _ -> inames
-  | C_STGhost inames _ -> inames
 
 let obs_of_comp (c:comp_st) : observability =
   match c with
   | C_ST _ -> Observable
+  | C_STGhost _ -> Neutral
   | C_STAtomic _ obs _ -> obs
-  | C_STGhost _ _ -> Unobservable
 
 (* Takes the two branches, with already matched effect,
 and matches their invariants (unless C_ST) *)
@@ -168,7 +168,8 @@ let match_inames
             obs_of_comp c_then' == obs_of_comp c_else'
          )
 = match c_then, c_else with
-  | C_ST _, C_ST _ ->
+  | C_ST _, C_ST _
+  | C_STGhost _, C_STGhost _ ->
     (| c_then, c_else, e_then_typing, e_else_typing |)
 
   | C_STAtomic inames1 obs1 stc_then, C_STAtomic inames2 obs2 stc_else ->
@@ -185,18 +186,6 @@ let match_inames
       (| C_STAtomic is _ stc_then, C_STAtomic is _ stc_else, e_then_typing, e_else_typing |)
     )
 
-  | C_STGhost inames1 stc_then, C_STGhost inames2 stc_else ->
-    if eq_tm inames1 inames2 then
-      (* easy case; an optimization *)
-      (| c_then, c_else, e_then_typing, e_else_typing |)
-    else (
-      let is = compute_iname_join inames1 inames2 in
-      let tok1 : prop_validity g_then (tm_inames_subset inames1 is) = RU.magic () in
-      let tok2 : prop_validity g_else (tm_inames_subset inames2 is) = RU.magic () in
-      let e_then_typing = T_Sub _ _ _ _ e_then_typing (STS_GhostInvs g_then stc_then inames1 is tok1) in
-      let e_else_typing = T_Sub _ _ _ _ e_else_typing (STS_GhostInvs g_else stc_else inames2 is tok2) in
-      (| C_STGhost is stc_then, C_STGhost is stc_else, e_then_typing, e_else_typing |)
-    )
 
 (* NB: g_then and g_else are equal except for containing one extra
 hypothesis according to which branch was taken. *)
@@ -298,6 +287,6 @@ let check
   in
 
   let d : st_typing_in_ctxt g pre (Some post_hint) =
-    (| _, c, T_If g b e1 e2 c _ hyp b_typing e1_typing e2_typing (E c_typing) |) in
+    (| _, c, T_If g b e1 e2 c hyp b_typing e1_typing e2_typing (E c_typing) |) in
 
   checker_result_for_st_typing d res_ppname
