pulse/lib/steel/pulse/Pulse.Readback.fst
@@ -28,6 +28,20 @@ let (let?) (f:option 'a) (g:'a -> option 'b) : option 'b =
   | None -> None
   | Some x -> g x
 
+let readback_observability (t:R.term)
+: option (obs:observability { elab_observability obs == t })
+= let open R in
+  match inspect_ln t with
+  | R.Tv_FVar fv ->
+    let fv_lid = inspect_fv fv in
+    if fv_lid = observable_lid
+    then Some Observable
+    else if fv_lid = unobservable_lid
+    then Some Unobservable
+    else if fv_lid = neutral_lid
+    then Some Neutral
+    else None
+  | _ -> None
 
 #push-options "--z3rlimit_factor 20"
 // TODO: FIXME: may be mark as opaque_to_smt
@@ -67,37 +81,40 @@ let try_readback_st_comp
               Some (c <: c:Pulse.Syntax.Base.comp{ elab_comp c == t })
             | _ -> None)
          | _ -> None
-    else if fv_lid = stt_atomic_lid || fv_lid = stt_unobservable_lid || fv_lid = stt_ghost_lid
+    else if fv_lid = stt_atomic_lid
     then match args with
-         | [res; opened; pre; post] ->
+         | [res; obs; opened; pre; post] ->
            (match inspect_ln (fst post) with
             | Tv_Abs b body ->
               let { qual=aq; attrs=attrs }
                   = inspect_binder b
               in    
               let? res' = readback_ty (fst res) in
+              let? obs' = readback_observability (fst obs) in
               let? opened' = readback_ty (fst opened) in
               let? pre' = readback_ty (fst pre) in
               let? post' = readback_ty body in
-              if fv_lid = stt_atomic_lid
-              then begin
-                assume (t == mk_stt_atomic_comp true u (fst res) (fst opened) (fst pre) (mk_abs (fst res) R.Q_Explicit body));
-                let c = C_STAtomic opened' Observable ({u; res=res'; pre=pre';post=post'}) in
-                Some (c <: c:Pulse.Syntax.Base.comp { elab_comp c == t })
-              end
-              else if fv_lid = stt_unobservable_lid
-              then begin
-                assume (t == mk_stt_atomic_comp false u (fst res) (fst opened) (fst pre) (mk_abs (fst res) R.Q_Explicit body));
-                let c = C_STAtomic opened' Unobservable ({u; res=res'; pre=pre';post=post'}) in
-                Some (c <: c:Pulse.Syntax.Base.comp { elab_comp c == t })
-              end
-              else begin
-                assume (t == mk_stt_ghost_comp u (fst res) (fst opened) (fst pre) (mk_abs (fst res) R.Q_Explicit body));
-                let c = C_STGhost opened' ({u; res=res'; pre=pre';post=post'}) in
-                Some (c <: c:Pulse.Syntax.Base.comp { elab_comp c == t })
-              end
+              assume (t == mk_stt_atomic_comp (fst obs) u (fst res) (fst opened) (fst pre) (mk_abs (fst res) R.Q_Explicit body));
+              let c = C_STAtomic opened' obs' ({u; res=res'; pre=pre';post=post'}) in
+              Some (c <: c:Pulse.Syntax.Base.comp { elab_comp c == t })
             | _ -> None)
          | _ -> None
+    else if fv_lid = stt_ghost_lid
+    then match args with
+         | [res; pre; post] ->
+           (match inspect_ln (fst post) with
+            | Tv_Abs b body ->
+              let { qual=aq; attrs=attrs }
+                  = inspect_binder b
+              in    
+              let? res' = readback_ty (fst res) in
+              let? pre' = readback_ty (fst pre) in
+              let? post' = readback_ty body in
+              assume (t == mk_stt_ghost_comp u (fst res) (fst pre) (mk_abs (fst res) R.Q_Explicit body));
+              let c = C_STGhost ({u; res=res'; pre=pre';post=post'}) in
+              Some (c <: c:Pulse.Syntax.Base.comp { elab_comp c == t })
+            | _ -> None)
+         | _ -> None    
     else None  
   | _ -> None
 #pop-options
