pulse/lib/steel/pulse/Pulse.Soundness.Return.fst
@@ -30,7 +30,7 @@ module WT = Pulse.Steel.Wrapper.Typing
 module LN = Pulse.Typing.LN
 
 #push-options "--z3rlimit_factor 4 --fuel 8 --ifuel 2"
-let return_soundess
+let return_soundness
   (#g:stt_env)
   (#t:st_term)
   (#c:comp)
@@ -133,10 +133,10 @@ let return_soundess
       assert (elab_comp c == mk_stt_comp ru rt elab_c_pre elab_c_post);
       elab_stt_equiv _ c _ _ pre_eq post_eq
     | STT_Atomic ->
-      assert (elab_comp c == mk_stt_atomic_comp false ru rt emp_inames_tm elab_c_pre elab_c_post);
+      assert (elab_comp c == mk_stt_atomic_comp Pulse.Steel.Wrapper.Typing.neutral_fv ru rt emp_inames_tm elab_c_pre elab_c_post);
       elab_statomic_equiv _ c _ _ pre_eq post_eq
     | STT_Ghost ->
-      assert (elab_comp c == mk_stt_ghost_comp ru rt emp_inames_tm elab_c_pre elab_c_post);
+      assert (elab_comp c == mk_stt_ghost_comp ru rt elab_c_pre elab_c_post);
       elab_stghost_equiv _ c _ _ pre_eq post_eq
   in
   match ctag, use_eq with
