pulse/lib/steel/pulse/Pulse.Syntax.Printer.fst
@@ -175,9 +175,9 @@ let ctag_to_string = function
 
 let observability_to_string =
   function
-  | Observable -> "atomic"
-  | Unobservable -> "unobservable"
-  | Neutral -> "neutral"
+  | Observable -> "Observable"
+  | Unobservable -> "Unobservable"
+  | Neutral -> "Neutral"
   
 let comp_to_string (c:comp)
   : T.Tac string
@@ -192,16 +192,15 @@ let comp_to_string (c:comp)
               (term_to_string s.post)
 
     | C_STAtomic inames obs s ->
-      sprintf "stt_%s %s %s (requires\n%s) (ensures\n%s)"
+      sprintf "stt_atomic %s #%s %s (requires\n%s) (ensures\n%s)"
+              (term_to_string s.res)
               (observability_to_string obs)
               (term_to_string inames)
-              (term_to_string s.res)
               (term_to_string s.pre)
               (term_to_string s.post)
 
-    | C_STGhost inames s ->
-      sprintf "stt_ghost %s %s (requires\n%s) (ensures\n%s)"
-              (term_to_string inames)
+    | C_STGhost s ->
+      sprintf "stt_ghost %s (requires\n%s) (ensures\n%s)"
               (term_to_string s.res)
               (term_to_string s.pre)
               (term_to_string s.post)
@@ -468,7 +467,7 @@ let tag_of_comp (c:comp) : T.Tac string =
   | C_ST _ -> "ST"
   | C_STAtomic i obs _ ->
     Printf.sprintf "%s %s" (observability_to_string obs) (term_to_string i)
-  | C_STGhost i _ ->
+  | C_STGhost _ ->
     "Ghost" 
     
 let rec print_st_head (t:st_term)
