pulse/lib/steel/pulse/Pulse.Typing.LN.fst
@@ -91,13 +91,13 @@ let open_comp_ln' (c:comp)
     | C_Tot t ->
       open_term_ln' t x i
 
-    | C_ST s ->
+    | C_ST s
+    | C_STGhost s ->
       open_term_ln' s.res x i;
       open_term_ln' s.pre x i;      
       open_term_ln' s.post x (i + 1)
 
-    | C_STAtomic n _ s
-    | C_STGhost n s ->    
+    | C_STAtomic n _ s ->    
       open_term_ln' n x i;    
       open_term_ln' s.res x i;
       open_term_ln' s.pre x i;      
@@ -410,13 +410,13 @@ let ln_weakening_comp (c:comp) (i j:int)
     | C_Tot t ->
       ln_weakening t i j
 
-    | C_ST s ->
+    | C_ST s
+    | C_STGhost s ->
       ln_weakening s.res i j;
       ln_weakening s.pre i j;      
       ln_weakening s.post (i + 1) (j + 1)
 
-    | C_STAtomic n _ s
-    | C_STGhost n s ->    
+    | C_STAtomic n _ s ->    
       ln_weakening n i j;    
       ln_weakening s.res i j;
       ln_weakening s.pre i j;      
@@ -616,13 +616,13 @@ let open_comp_ln_inv' (c:comp)
     | C_Tot t ->
       open_term_ln_inv' t x i
 
-    | C_ST s ->
+    | C_ST s
+    | C_STGhost s ->
       open_term_ln_inv' s.res x i;
       open_term_ln_inv' s.pre x i;      
       open_term_ln_inv' s.post x (i + 1)
 
-    | C_STAtomic n _ s
-    | C_STGhost n s ->    
+    | C_STAtomic n _ s ->    
       open_term_ln_inv' n x i;    
       open_term_ln_inv' s.res x i;
       open_term_ln_inv' s.pre x i;      
@@ -831,13 +831,13 @@ let close_comp_ln' (c:comp)
     | C_Tot t ->
       close_term_ln' t x i
 
-    | C_ST s ->
+    | C_ST s
+    | C_STGhost s ->
       close_term_ln' s.res x i;
       close_term_ln' s.pre x i;      
       close_term_ln' s.post x (i + 1)
 
-    | C_STAtomic n _ s
-    | C_STGhost n s ->    
+    | C_STAtomic n _ s ->    
       close_term_ln' n x i;    
       close_term_ln' s.res x i;
       close_term_ln' s.pre x i;      
@@ -1088,14 +1088,10 @@ let rec st_sub_ln #g #c1 #c2 (d:st_sub g c1 c2)
     (decreases d)
   = match d with
     | STS_Refl _ _ -> ()
+
     | STS_Trans _ _ _ _ d1 d2 ->
       st_sub_ln d1;
       st_sub_ln d2
-
-    | STS_GhostInvs g stc is1 is2 tok ->
-      prop_valid_must_be_ln g (tm_inames_subset is1 is2) tok;
-      (* This should be easy-ish to prove, since is2 is a subterm *)
-      assume (ln (tm_inames_subset is1 is2) ==> ln is2)
 
     | STS_AtomicInvs g stc is1 is2 _ _ tok ->
       prop_valid_must_be_ln g (tm_inames_subset is1 is2) tok;
@@ -1121,9 +1117,9 @@ let comp_typing_ln (#g:_) (#c:_) (#u:_) (d:comp_typing g c u)
 
   match d with
   | CT_Tot _ _ _ t_typing -> tot_or_ghost_typing_ln t_typing
-  | CT_ST _ _ st_typing -> st_comp_typing_ln st_typing
-  | CT_STAtomic _ _ _ _ inames_typing st_typing
-  | CT_STGhost _ _ _ inames_typing st_typing ->
+  | CT_ST _ _ st_typing
+  | CT_STGhost _ _ st_typing -> st_comp_typing_ln st_typing
+  | CT_STAtomic _ _ _ _ inames_typing st_typing ->
     tot_or_ghost_typing_ln inames_typing;
     st_comp_typing_ln st_typing
 
@@ -1240,7 +1236,7 @@ let rec st_typing_ln (#g:_) (#t:_) (#c:_)
     | T_GhostBind _ _ _ _ _ _ _ _ _ _ ->
       st_typing_ln_tot_or_ghost_bind d st_typing_ln
 
-    | T_If _ _ _ _ _ _ _ tb d1 d2 _ ->
+    | T_If _ _ _ _ _ _ tb d1 d2 _ ->
       tot_or_ghost_typing_ln tb;
       st_typing_ln d1;
       st_typing_ln d2
