pulse/share/steel/examples/pulse/bug-reports/BugGhostReturn.fst
@@ -1,0 +1,62 @@
+module BugGhostReturn
+open Pulse.Lib.Pervasives
+
+assume
+val extract (#a:Type) (x:squash a) : erased a
+
+let pextract (#a:Type)
+: stt_ghost (erased a) emp_inames (pure (squash a)) (fun _ -> emp)
+= bind_sttg (elim_pure_explicit (squash a))
+            (fun (x:squash a) -> 
+                return_stt_ghost_noeq (extract x) (fun _ -> emp))
+
+let join (#a:Type)
+: Lemma (requires (squash (squash a)))
+        (ensures (squash a))
+        [SMTPat (squash (squash a))]
+= ()        
+// = FStar.Squash.join_squash #a ()
+
+let psquash (a:Type u#a) : prop = squash a
+
+```pulse
+fn pextract' (#a:Type u#0)
+requires pure (squash a)
+returns i:erased a
+ensures emp
+{
+  let pf = elim_pure_explicit (psquash a);
+  let pf : squash a = FStar.Squash.join_squash pf;
+  let i = extract #a pf;
+  i
+}
+```
+
+assume
+val p (#a:Type) (x:a) : prop
+
+assume
+val some_lemma (#a:Type) (x:a)
+  : Lemma (p x)
+
+```pulse
+fn use_some_lemma (#a:Type u#0) (x:a)
+requires emp
+ensures pure (p x)
+{
+  some_lemma x;
+  ()
+}
+```
+
+// [@@expect_failure]
+```pulse
+ghost
+fn use_some_lemma_ghost (#a:Type u#0) (x:a)
+requires emp
+ensures pure (p x)
+{
+  some_lemma x;
+  ()
+}
+```
